Most recent, partially complete Algebraic table proofs

BranchTable_v3.v
@@ -300,13 +300,14 @@ Fixpoint AssociationGet {key V: Type} (k: key) (t: list(key * V)) (default: V) `
       |Coq.Lists.List.cons (k', v) t' => 
         if k =? k' then v else AssociationGet k t' default
       end.  
+
 Require Import Fin.
 
 Definition nat_to_fin (n : nat) (H : 0 < n) : Fin.t n :=
   Fin.of_nat_lt H.
 
 #[export] Instance HAMTTable (key V:Type) (n: nat) (f: key -> nat) (default:V) 
-`{EqDec key} (Hvalid1: forall k, f k < n) (Hvalid2: forall k, 0 < k): Table key V default :=
+`{EqDec key} (Hvalid1: forall k, f k < n) : Table key V default :=
   {
     table := MyRecord key V n; 
     empty := createEmptyRecord key V n;
@@ -318,10 +319,8 @@ Definition nat_to_fin (n : nat) (H : 0 < n) : Fin.t n :=
       | _ => default
       end;
     set k v t := 
-      let k' := f k in 
       let fin_k' := Fin.of_nat_lt (Hvalid1 k) in
-      let fin_n := nat_to_fin n (Hvalid2 n) in
-      let new_bitmap := upd_nth fin_n true t.(bitmap key V n) in 
+      let new_bitmap := upd_nth fin_k' true t.(bitmap key V n) in 
       let new_array := upd_nth fin_k' (Coq.Lists.List.cons (k, v) (nth t.(array key V n) fin_k')) t.(array key V n)
     in
     {|
@@ -334,14 +333,80 @@ Definition nat_to_fin (n : nat) (H : 0 < n) : Fin.t n :=
 Lemma const_false : forall (key: Type) (k: key) (n : nat) (f: key -> nat) (H : forall k, f k < n), 
 (const false n)[@of_nat_lt (H k)] = false.
 Proof. 
-intros. unfold of_nat_lt. intros.  
+intros. apply const_nth.
+Qed.  
+
+From Coq Require Export Vectors.Vector.
+Import VectorNotations.
+
+Lemma upd_nth' : forall (key V : Type) (f: key -> nat) (k: key) (n: nat) 
+(v : t V n) (x: V) (H2: forall l : key, f l < n),
+(upd_nth (Fin.of_nat_lt (H2 k)) x v)[@of_nat_lt (H2 k)] = x.
+Proof.
+intros. unfold upd_nth. apply nth_order_replace_eq.
+Qed.
+
+From Coq Require Export Arith.PeanoNat.
+From Coq Require Export Logic.ProofIrrelevance.
+
+Lemma nat_to_fin_eq : forall (n m p : nat) (Hn : n < p) (Hm : m < p),
+  n = m -> Fin.of_nat_lt Hn = Fin.of_nat_lt Hm.
+Proof.
+  intros n m p Hn Hm Heq.
+  subst m.
+  f_equal.
+  apply proof_irrelevance.
+Qed.
+
+Lemma AG_equiv : forall (key V: Type) (f : key -> nat) (n: nat) (t: MyRecord key V n) (l: list (key * V)) (k k': key) (def: V) (v: V) (H: forall k : key, f k < n ) `{EqDec key}, 
+k <> k' -> AssociationGet k' (replace (array key V n t)(of_nat_lt (H k'))(Coq.Lists.List.cons (k, v) l))[@
+ of_nat_lt (H k')] def = AssociationGet k' l def.
+Proof. 
+  Admitted. 
+
+Lemma upd_AG : forall {key V: Type} (k k1: key) (x: V) (t: list(key * V)) (default: V) `{EqDec key},
+  k <> k1 -> AssociationGet k (Coq.Lists.List.cons (k1, x) t) default = AssociationGet k t default.
+Proof. intros. simpl. inversion H0. destruct (eqb_reflect0 k k1). contradiction. reflexivity.
+  Qed.
+  
+Lemma upd_nth_neq : forall (key V: Type) (f : key -> nat) (n: nat) (t: MyRecord key V n) (k k': key) (H: forall k : key, f k < n ) `{EqDec key} `{Eq key}, 
+f k <> f k' -> (upd_nth (of_nat_lt (H k)) true (bitmap key V n t))[@of_nat_lt (H k')] = (bitmap key V n t)[@of_nat_lt (H k')].
+Proof.
+Admitted. 
+
+Lemma upd_nth_neq_H : forall (key V: Type) (f : key -> nat) (k: key) (v: V) (n: nat) (t: MyRecord key V n) (k k': key) (H: forall k : key, f k < n ) `{EqDec key} `{Eq key}, 
+  f k <> f k' -> (upd_nth (of_nat_lt (H k)) ((k, v) :: (array key V n t)[@of_nat_lt (H k)])%list
+ (array key V n t))[@of_nat_lt (H k')] = (array key V n t)[@of_nat_lt (H k')].
+  Proof.
+Admitted. 
 
 #[export] Instance FunHAMTTableAlgebraic (key V:Type) (n: nat) 
-(default:V) (f: key -> nat) (Hvalid2: forall k, 0 < k) 
+(default:V) (f: key -> nat) (H: forall l : key, f l < n)
 (Hvalid1: forall k, f k < n) `{EqDec key} :
-  AlgebraicTable (HAMTTable key V n f default Hvalid1 Hvalid2).
+  AlgebraicTable (HAMTTable key V n f default H).
 Proof.
   constructor.
-  - intros. unfold get, HAMTTable, createEmptyRecord, AssociationGet.
-  simpl.    
-  Admitted. 
+  - intros. unfold get, empty, HAMTTable. rewrite -> const_false. auto.
+  - intros. unfold get, set, HAMTTable. simpl. rewrite -> upd_nth'. rewrite -> upd_nth'.
+  simpl. inversion H1. destruct (eqb_reflect0 k k). auto. destruct n0. reflexivity.
+  - intros. unfold get, set, HAMTTable. simpl. destruct (Nat.eq_dec (f k) (f k')) as [Heq_nat | Hneq_nat]. 
+  assert (of_nat_lt (H k) = of_nat_lt (H k')). { simpl. apply nat_to_fin_eq. apply Heq_nat. }
+  rewrite -> H3. 
+    * destruct ((bitmap key V n t)[@of_nat_lt (H k')]).
+      ** rewrite -> upd_nth'. simpl. destruct ((array key V n t)[@of_nat_lt (H k')]).
+        *** simpl. unfold upd_nth. simpl. rewrite -> AG_equiv. simpl. reflexivity. apply H2.
+        *** unfold upd_nth. rewrite -> AG_equiv. reflexivity. apply H2.
+      ** simpl. rewrite upd_nth'. simpl. destruct ((array key V n t)[@of_nat_lt (H k')]).
+        *** simpl. unfold upd_nth. rewrite -> AG_equiv. auto. auto.
+        *** simpl. unfold upd_nth. rewrite -> AG_equiv. 
+        (* first destruct implies l must also be empty*) admit. auto.
+    * rewrite -> upd_nth_neq with (H0 := H0). 
+    rewrite -> upd_nth_neq_H with (H0 := H0). reflexivity.
+    repeat auto. auto. auto. auto. auto. auto. auto.
+Admitted.       (* hash not equal case, shouldn't even update the lists *)                            
+      
+    
+    
+    
+  
+
